## Derivation of Regression Model and Coefficient Mapping

**1. Theoretical Model:**

The starting equation is:
$$Y = \text{Constant} + (A_0 + A_1 h) ( (1 - \alpha) + \alpha (\psi + \psi_0 + \phi \log(h)))$$
Given $\psi = \psi_1 \text{Tele}$, we substitute it in:
$$Y = \text{Constant} + (A_0 + A_1 h) ( (1 - \alpha) + \alpha (\psi_1 \text{Tele} + \psi_0 + \phi \log(h)))$$

**2. Expansion of the Model:**

We need to multiply out the terms to identify the components that will form our regression variables.

*   First, distribute $\alpha$ inside the second parenthesis:
    $$(A_0 + A_1 h) ( 1 - \alpha + \alpha \psi_1 \text{Tele} + \alpha \psi_0 + \alpha \phi \log(h) )$$
*   Next, distribute the $(A_0 + A_1 h)$ term across the terms in the second parenthesis:
    $$ Y = \text{Constant} + \left[ A_0(1) + A_0(-\alpha) + A_0(\alpha \psi_1 \text{Tele}) + A_0(\alpha \psi_0) + A_0(\alpha \phi \log(h)) \right] \\ + \left[ A_1 h(1) + A_1 h(-\alpha) + A_1 h(\alpha \psi_1 \text{Tele}) + A_1 h(\alpha \psi_0) + A_1 h(\alpha \phi \log(h)) \right] $$
*   Simplify and group terms based on the original parameters:
    $$ Y = \text{Constant} + A_0 - A_0 \alpha + A_0 \alpha \psi_1 \text{Tele} + A_0 \alpha \psi_0 + A_0 \alpha \phi \log(h) \\ + A_1 h - A_1 h \alpha + A_1 h \alpha \psi_1 \text{Tele} + A_1 h \alpha \psi_0 + A_1 h \alpha \phi \log(h) $$

**3. Rearranging for Regression:**

Now, we group terms based on the *observable* variables and their combinations ($h, \alpha, \text{Tele}, \log(h)$) to fit the linear regression structure $Y = \beta_0 + \sum \beta_i X_i + \epsilon$.

*   **Constant Term:** $\text{Constant} + A_0$
*   **Term involving $h$:** $A_1 h$
*   **Term involving $\alpha$:** $-A_0 \alpha + A_0 \alpha \psi_0 = A_0(\psi_0 - 1) \alpha$
*   **Term involving $h \alpha$:** $-A_1 h \alpha + A_1 h \alpha \psi_0 = A_1(\psi_0 - 1) (h \alpha)$
*   **Term involving $\alpha \text{Tele}$:** $A_0 \psi_1 (\alpha \text{Tele})$
*   **Term involving $h \alpha \text{Tele}$:** $A_1 \psi_1 (h \alpha \text{Tele})$
*   **Term involving $\alpha \log(h)$:** $A_0 \phi (\alpha \log(h))$
*   **Term involving $h \alpha \log(h)$:** $A_1 \phi (h \alpha \log(h))$

Combining these gives:
$$ Y = (\text{Constant} + A_0) + A_1 h + A_0(\psi_0 - 1) \alpha + A_1(\psi_0 - 1) (h \alpha) \\ + A_0 \psi_1 (\alpha \text{Tele}) + A_1 \psi_1 (h \alpha \text{Tele}) + A_0 \phi (\alpha \log(h)) + A_1 \phi (h \alpha \log(h)) $$

**4. Regression Model Formulation:**

Based on the rearranged equation, we define the regression variables ($X_i$) and formulate the model:
$$ Y = \beta_0 + \beta_1 X_1 + \beta_2 X_2 + \beta_3 X_3 + \beta_4 X_4 + \beta_5 X_5 + \beta_6 X_6 + \beta_7 X_7 + \epsilon $$
where:
*   $X_1 = h$
*   $X_2 = \alpha$
*   $X_3 = h \alpha$
*   $X_4 = \alpha \text{Tele}$
*   $X_5 = h \alpha \text{Tele}$
*   $X_6 = \alpha \log(h)$
*   $X_7 = h \alpha \log(h)$
*   $\beta_0$ is the intercept term.
*   $\epsilon$ is the error term.

**5. Mapping Theoretical Parameters to Regression Coefficients:**

By comparing the rearranged theoretical equation with the regression model, we establish the following relationships:

*   $\beta_0 = \text{Constant} + A_0$
*   $\beta_1 = A_1$
*   $\beta_2 = A_0 (\psi_0 - 1)$
*   $\beta_3 = A_1 (\psi_0 - 1)$
*   $\beta_4 = A_0 \psi_1$
*   $\beta_5 = A_1 \psi_1$
*   $\beta_6 = A_0 \phi$
*   $\beta_7 = A_1 \phi$

**6. Solving for Original Parameters:**

After estimating the regression coefficients ($\hat{\beta}_0, \hat{\beta}_1, ..., \hat{\beta}_7$), we can solve for the original parameters.

1.  **Solve for $A_1$:**
    $$ A_1 = \hat{\beta}_1 $$
    *(Requires $\hat{\beta}_1 \neq 0$ for subsequent steps involving division by $A_1$).*

2.  **Solve for $\psi_0$:** Using the equation for $\beta_3$:
    $\hat{\beta}_3 = A_1 (\psi_0 - 1) = \hat{\beta}_1 (\psi_0 - 1)$
    $\psi_0 - 1 = \frac{\hat{\beta}_3}{\hat{\beta}_1}$
    $$ \psi_0 = \frac{\hat{\beta}_3}{\hat{\beta}_1} + 1 $$

3.  **Solve for $\psi_1$:** Using the equation for $\beta_5$:
    $\hat{\beta}_5 = A_1 \psi_1 = \hat{\beta}_1 \psi_1$
    $$ \psi_1 = \frac{\hat{\beta}_5}{\hat{\beta}_1} $$

4.  **Solve for $\phi$:** Using the equation for $\beta_7$:
    $\hat{\beta}_7 = A_1 \phi = \hat{\beta}_1 \phi$
    $$ \phi = \frac{\hat{\beta}_7}{\hat{\beta}_1} $$

5.  **Solve for $A_0$:** We can use several equations. Using the equation for $\beta_4$:
    $\hat{\beta}_4 = A_0 \psi_1$. Substitute the expression for $\psi_1$:
    $\hat{\beta}_4 = A_0 \left( \frac{\hat{\beta}_5}{\hat{\beta}_1} \right)$
    $$ A_0 = \frac{\hat{\beta}_1 \hat{\beta}_4}{\hat{\beta}_5} $$
    *(Requires $\hat{\beta}_5 \neq 0$).*
    *Alternatively*, using $\beta_2 = A_0 (\psi_0 - 1)$:
    $\hat{\beta}_2 = A_0 \left( \frac{\hat{\beta}_3}{\hat{\beta}_1} \right)$
    $$ A_0 = \frac{\hat{\beta}_1 \hat{\beta}_2}{\hat{\beta}_3} $$
    *(Requires $\hat{\beta}_3 \neq 0$).*
    *Alternatively*, using $\beta_6 = A_0 \phi$:
    $\hat{\beta}_6 = A_0 \left( \frac{\hat{\beta}_7}{\hat{\beta}_1} \right)$
    $$ A_0 = \frac{\hat{\beta}_1 \hat{\beta}_6}{\hat{\beta}_7} $$
    *(Requires $\hat{\beta}_7 \neq 0$).*
    **(Important Note:** For the theoretical model to hold, these different ways of calculating $A_0$ must yield the same result. This implies testable constraints on the regression coefficients: $\frac{\hat{\beta}_4}{\hat{\beta}_5} = \frac{\hat{\beta}_2}{\hat{\beta}_3} = \frac{\hat{\beta}_6}{\hat{\beta}_7}$. This reflects the ratio $A_0/A_1$. Significant deviations suggest the model structure might be incorrect.)*

6.  **Solve for Constant:** Using the equation for $\beta_0$:
    $\hat{\beta}_0 = \text{Constant} + A_0$. Substitute the expression for $A_0$ (using one of the derived forms, e.g., the first one):
    $$ \text{Constant} = \hat{\beta}_0 - A_0 = \hat{\beta}_0 - \frac{\hat{\beta}_1 \hat{\beta}_4}{\hat{\beta}_5} $$

**Summary:**

To estimate the parameters of the model $Y = \text{Constant} + (A_0 + A_1 h) ( (1 - \alpha) + \alpha (\psi_1 \text{Tele} + \psi_0 + \phi \log(h)))$, run the following linear regression:

$Y = \beta_0 + \beta_1 h + \beta_2 \alpha + \beta_3 (h \alpha) + \beta_4 (\alpha \text{Tele}) + \beta_5 (h \alpha \text{Tele}) + \beta_6 (\alpha \log(h)) + \beta_7 (h \alpha \log(h)) + \epsilon$

The original parameters are recovered from the estimated coefficients $\hat{\beta}_i$ as:

*   $A_1 = \hat{\beta}_1$
*   $\psi_0 = (\hat{\beta}_3 / \hat{\beta}_1) + 1$
*   $\psi_1 = \hat{\beta}_5 / \hat{\beta}_1$
*   $\phi = \hat{\beta}_7 / \hat{\beta}_1$
*   $A_0 = \hat{\beta}_1 \hat{\beta}_4 / \hat{\beta}_5$ (or using $\beta_2/\beta_3$ or $\beta_6/\beta_7$)
*   $\text{Constant} = \hat{\beta}_0 - (\hat{\beta}_1 \hat{\beta}_4 / \hat{\beta}_5)$ (or using the corresponding expression for $A_0$)

**Caveats:**
*   The recovery of parameters involves division by $\hat{\beta}_1$, $\hat{\beta}_3$, $\hat{\beta}_5$, and $\hat{\beta}_7$. Ensure these estimates are statistically significantly different from zero and handle potential numerical instability if they are very small.
*   The validity of the original model structure imposes cross-equation restrictions on the $\beta$ coefficients (i.e., $\beta_2/\beta_3 = \beta_4/\beta_5 = \beta_6/\beta_7$). These can be tested statistically after estimation.